research/lean_only_proto/DumbContracts/Lang.lean
@@ -1,0 +1,46 @@
+import DumbContracts.Core
+
+namespace DumbContracts.Lang
+
+inductive Expr where
+  | lit : Nat -> Expr
+  | var : String -> Expr
+  | add : Expr -> Expr -> Expr
+  | sub : Expr -> Expr -> Expr
+  | mul : Expr -> Expr -> Expr
+  | div : Expr -> Expr -> Expr
+  | eq : Expr -> Expr -> Expr
+  | lt : Expr -> Expr -> Expr
+  | gt : Expr -> Expr -> Expr
+  | and : Expr -> Expr -> Expr
+  | or : Expr -> Expr -> Expr
+  | not : Expr -> Expr
+  | sload : Expr -> Expr
+  deriving Repr
+
+inductive Stmt where
+  | skip : Stmt
+  | seq : Stmt -> Stmt -> Stmt
+  | let_ : String -> Expr -> Stmt -> Stmt
+  | assign : String -> Expr -> Stmt
+  | if_ : Expr -> Stmt -> Stmt -> Stmt
+  | sstore : Expr -> Expr -> Stmt
+  | revert : Stmt
+  | return_ : Expr -> Stmt
+  deriving Repr
+
+structure Fun where
+  name : String
+  args : List String
+  body : Stmt
+  ret : Option String
+  deriving Repr
+
+structure Program where
+  funs : List Fun
+  entry : Stmt
+  deriving Repr
+
+notation:50 a " ;; " b => Stmt.seq a b
+
+end DumbContracts.Lang
