research/lean_only_proto/lakefile.lean
@@ -5,3 +5,6 @@ package dumbcontracts where
   moreLeanArgs := #["-Dlinter.unusedVariables=false"]
 
 lean_lib DumbContracts
+
+lean_exe dumbcontracts where
+  root := `Main
